More progress towards closing the gap between WP and bisim with leaps.

deps/poulet4/lib/P4automata/Bisimulations/WPLeapsProofs.v
@@ -9,6 +9,7 @@ Require Import Poulet4.P4automata.ConfRel.
 Require Import Poulet4.Relations.
 Require Import Poulet4.P4automata.WPProofs.
 Require Import Poulet4.P4automata.Bisimulations.Leaps.
+Require Import Poulet4.P4automata.Bisimulations.LeapsProofs.
 Require Import Poulet4.P4automata.Bisimulations.AlgorithmicLeaps.
 Require Import Poulet4.P4automata.Bisimulations.AlgorithmicLeapsProofs.
 Require Import Poulet4.P4automata.Bisimulations.WPLeaps.
@@ -41,8 +42,7 @@ Section WPLeapsProofs.
 
   Notation conf := (configuration (P4A.interp a)).
 
-  Variable (top: rel conf).
-  Variable (top_closed: forall x y b, top x y -> top (step x b) (step y b)).
+  Definition top q1 q2 := In (conf_to_state_template q1, conf_to_state_template q2) r.
 
   Notation "⟦ x ⟧" := (interp_crel a top x).
   Notation "⦇ x ⦈" := (interp_conf_rel a x).
@@ -136,27 +136,33 @@ Section WPLeapsProofs.
     induction R; cbn; intuition.
   Qed.
 
-  Lemma interp_crel_nodup:
-    forall R (q1 q2: conf),
-      ⟦R⟧ q1 q2 <->
-      ⟦nodup (conf_rel_eq_dec (a := a)) R⟧ q1 q2.
-  Proof.
-  Admitted.
+  Opaque top.
 
   Lemma interp_crel_quantify:
     forall R (q1 q2: conf),
       ⟦R⟧ q1 q2 <->
       top q1 q2 /\ (forall phi, In phi R -> ⦇phi⦈ q1 q2).
   Proof.
-  Admitted.
+    intros; induction R.
+    - intuition.
+    - rewrite interp_crel_cons, IHR; intuition.
+      destruct H4; subst; intuition.
+  Qed.
 
-  Hypothesis top_versus_reachable:
-    forall q1 q2,
-      top q1 q2 ->
-      In (conf_to_state_template q1, conf_to_state_template q2) r.
+  Transparent top.
+
+  Lemma interp_crel_nodup:
+    forall R (q1 q2: conf),
+      ⟦R⟧ q1 q2 <->
+      ⟦nodup (conf_rel_eq_dec (a := a)) R⟧ q1 q2.
+  Proof.
+    intros.
+    repeat rewrite interp_crel_quantify.
+    now setoid_rewrite nodup_In.
+  Qed.
 
   Lemma init_vs_accepting:
-    forall (q1 q2: conf) s1 s2,
+    forall (q1 q2: conf),
       ⟦mk_init _ _ _ _ (length (valid_state_pairs a)) s1 s2⟧ q1 q2 ->
       (accepting q1 <-> accepting q2).
   Proof.
@@ -166,11 +172,377 @@ Section WPLeapsProofs.
     unfold mk_partition in H0.
     rewrite interp_crel_quantify in H0.
     destruct H0.
-    apply top_versus_reachable in H0.
+    unfold top in H0.
     unfold r in H0.
     unfold accepting.
     split; intros.
-  Admitted.
+    assert (~ not_equally_accepting S1 S2 H a (conf_to_state_template q1, conf_to_state_template q2) = true).
+    intro.
+    assert (⦇ mk_rel S1 S2 H a (conf_to_state_template q1, conf_to_state_template q2) ⦈ q1 q2).
+    apply H1.
+    apply in_map.
+    rewrite filter_In.
+    split; auto.
+    unfold mk_rel in H4.
+    unfold interp_conf_rel in H4.
+    vm_compute in H4.
+    apply H4.
+    intuition.
+    exact tt.
+    rewrite Bool.not_true_iff_false in H3.
+    unfold not_equally_accepting in H3.
+    unfold conf_to_state_template in H3.
+    simpl in H3.
+    rewrite H2 in H3.
+    destruct (conf_state q2).
+    discriminate.
+    destruct b.
+    reflexivity.
+    discriminate.
+    assert (~ not_equally_accepting S1 S2 H a (conf_to_state_template q1, conf_to_state_template q2) = true).
+    intro.
+    assert (⦇ mk_rel S1 S2 H a (conf_to_state_template q1, conf_to_state_template q2) ⦈ q1 q2).
+    apply H1.
+    apply in_map.
+    rewrite filter_In.
+    split; auto.
+    unfold mk_rel in H4.
+    unfold interp_conf_rel in H4.
+    vm_compute in H4.
+    apply H4.
+    intuition.
+    exact tt.
+    rewrite Bool.not_true_iff_false in H3.
+    unfold not_equally_accepting in H3.
+    unfold conf_to_state_template in H3.
+    simpl in H3.
+    rewrite H2 in H3.
+    destruct (conf_state q1).
+    discriminate.
+    destruct b.
+    reflexivity.
+    discriminate.
+  Qed.
+
+  Lemma reachable_states_closed r (p1 p2: Reachability.state_pair a):
+    (forall p, List.In p r -> valid_state_pair p) ->
+    List.In p1 (reachable_states' (length (valid_state_pairs a)) r) ->
+    List.In p2 (reachable_step [p1]) ->
+    List.In p2 (reachable_states' (length (valid_state_pairs a)) r).
+  Proof.
+    intros.
+    apply reachable_states_bound with (fuel := Datatypes.S (length (valid_state_pairs a))); auto.
+    unfold reachable_states'.
+    fold (reachable_states' (length (valid_state_pairs a)) r).
+    revert H2; apply reachable_step_mono.
+    unfold incl; intros.
+    destruct H2; try contradiction; now subst.
+  Qed.
+
+  Lemma follow_false q bs:
+    conf_state q = inr false ->
+    conf_state (follow (a := P4A.interp a) q bs) = inr false.
+  Proof.
+    revert q; induction bs; intros.
+    - now autorewrite with follow.
+    - autorewrite with follow.
+      apply IHbs.
+      unfold step.
+      destruct (Compare_dec.le_lt_dec _ _).
+      + simpl.
+        match goal with
+        | |- context [ (WP.P4A.P4A.update' _ _ ?t _) ] =>
+          generalize t
+        end.
+        intros.
+        destruct (WP.P4A.P4A.conf_state q).
+        * discriminate.
+        * autorewrite with update'.
+          autorewrite with transitions'.
+          reflexivity.
+      + simpl.
+        apply H0.
+  Qed.
+
+  Lemma buf_len_halted q b:
+    conf_state q = inr b ->
+    conf_buf_len (a := P4A.interp a) q = 0.
+  Proof.
+    intros.
+    destruct q.
+    simpl in *.
+    rewrite H0 in conf_buf_sane.
+    autorewrite with size' in conf_buf_sane.
+    Lia.lia.
+  Qed.
+
+  Lemma foo q1 bs:
+    1 <= length bs <= configuration_room_left q1 ->
+    In (conf_to_state_template (follow q1 bs))
+      (advance (a := a)
+         (length bs)
+         (conf_to_state_template q1) (st_state (conf_to_state_template q1))).
+  Proof.
+    intros.
+    unfold advance.
+    unfold conf_to_state_template at 2; simpl.
+    destruct (conf_state q1) eqn:?.
+    - unfold configuration_room_left in H0.
+      rewrite Heqs in H0.
+      autorewrite with size' in H0.
+      destruct (Compare_dec.le_gt_dec _ _).
+      + simpl in H0.
+        assert (P4A.size (S := Reachability.S S1 S2) a s = conf_buf_len q1 + length bs) by Lia.lia.
+        clear l.
+        destruct H0.
+        clear H2.
+        revert q1 Heqs H1.
+        induction bs; intros.
+        * simpl in H1.
+          pose proof (conf_buf_sane q1).
+          rewrite Heqs in H2.
+          autorewrite with size' in H2.
+          simpl in H2.
+          Lia.lia.
+        * destruct bs.
+          -- autorewrite with follow.
+             simpl in H1.
+             unfold step.
+             destruct (Compare_dec.le_lt_dec _ _).
+             ++ simpl.
+                match goal with
+                | |- context [ WP.P4A.P4A.update' _ _ ?t _ ] =>
+                  generalize t
+                end; intros.
+                unfold conf_to_state_template.
+                simpl.
+                apply in_map_iff.
+                eexists.
+                split.
+                reflexivity.
+                destruct (WP.P4A.P4A.conf_state q1); [|discriminate].
+                autorewrite with update'.
+                autorewrite with transitions'.
+                unfold possible_next_states.
+                unfold WP.P4A.P4A.transitions.
+                simpl.
+                unfold P4A.transitions.
+                unfold P4A.eval_trans.
+                inversion Heqs.
+                subst.
+                destruct (P4A.st_trans _).
+                apply in_eq.
+                induction cases.
+                simpl.
+                left; reflexivity.
+                simpl P4A.eval_sel.
+                destruct (P4A.match_pat _ _ _ _).
+                rewrite map_cons.
+                apply in_cons.
+                apply in_eq.
+                rewrite map_cons.
+                destruct IHcases.
+                rewrite H2 at 2.
+                apply in_eq.
+                apply in_cons.
+                apply in_cons.
+                apply H2.
+             ++ exfalso.
+                rewrite Heqs in l.
+                autorewrite with size' in l.
+                simpl in l.
+                Lia.lia.
+          -- rewrite follow_equation_2.
+             apply IHbs.
+             ++ simpl.
+                Lia.lia.
+             ++ unfold step.
+                destruct (Compare_dec.le_lt_dec _ _).
+                ** exfalso.
+                   rewrite Heqs in l.
+                   autorewrite with size' in l.
+                   simpl in l.
+                   simpl in H1.
+                   Lia.lia.
+                ** now simpl.
+             ++ unfold step.
+                destruct (Compare_dec.le_lt_dec _ _).
+                ** exfalso.
+                   rewrite Heqs in l.
+                   autorewrite with size' in l.
+                   simpl in l.
+                   simpl in H1.
+                   Lia.lia.
+                ** simpl in *.
+                   Lia.lia.
+      + clear H0; revert q1 s Heqs g; induction bs; intros.
+        * autorewrite with follow.
+          left.
+          unfold conf_to_state_template.
+          now f_equal.
+        * autorewrite with follow.
+          replace (conf_buf_len q1 + length (a0 :: bs))
+          with ((1 + conf_buf_len q1) + length bs) by (simpl; Lia.lia).
+          replace (1 + conf_buf_len q1) with (conf_buf_len (δ q1 a0)).
+          apply IHbs.
+          -- unfold step.
+             destruct (Compare_dec.le_lt_dec _ _).
+             ++ exfalso.
+                rewrite Heqs in l.
+                autorewrite with size' in l.
+                simpl in l, g.
+                Lia.lia.
+             ++ now simpl.
+          -- unfold step.
+             destruct (Compare_dec.le_lt_dec _ _).
+             ++ exfalso.
+                rewrite Heqs in l.
+                autorewrite with size' in l.
+                simpl in l, g.
+                Lia.lia.
+             ++ simpl in *.
+                Lia.lia.
+          -- unfold step.
+             destruct (Compare_dec.le_lt_dec _ _).
+             ++ exfalso.
+                rewrite Heqs in l.
+                autorewrite with size' in l.
+                simpl in l, g.
+                Lia.lia.
+             ++ now simpl.
+    - destruct bs.
+      + simpl in H0; Lia.lia.
+      + autorewrite with follow.
+        destruct q1.
+        simpl in Heqs.
+        unfold step.
+        simpl.
+        destruct (Compare_dec.le_lt_dec _ _).
+        destruct (conf_state).
+        discriminate.
+        inversion Heqs.
+        autorewrite with transitions'.
+        left.
+        unfold conf_to_state_template.
+        f_equal.
+        rewrite follow_false.
+        reflexivity.
+        simpl.
+        reflexivity.
+        rewrite buf_len_halted with (b := false).
+        reflexivity.
+        apply follow_false.
+        simpl.
+        reflexivity.
+        right.
+        rewrite Heqs in l.
+        autorewrite with size' in l.
+        Lia.lia.
+  Qed.
+
+  Lemma top_closed q1 q2 bs:
+    length bs = reads_left (conf_to_state_template q1, conf_to_state_template q2) ->
+    top q1 q2 ->
+    top (follow q1 bs) (follow q2 bs).
+  Proof.
+    unfold top, r, reachable_states; intros.
+    eapply reachable_states_closed.
+    - intros.
+      destruct H2; try contradiction.
+      subst.
+      unfold valid_state_pair, valid_state_template; simpl.
+      split; apply Syntax.t_has_extract.
+    - exact H1.
+    - unfold reachable_step.
+      apply nodup_In.
+      simpl.
+      rewrite app_nil_r, in_app_iff; left.
+      unfold reachable_pair_step.
+      unfold reachable_pair_step'.
+      apply in_prod.
+      + rewrite <- H0.
+        simpl.
+        destruct (conf_state q1) eqn:?.
+        * rewrite <- Heqs.
+          apply foo.
+          split.
+          -- rewrite H0.
+             unfold reads_left; simpl.
+             pose proof (conf_buf_sane q1).
+             pose proof (conf_buf_sane q2).
+             destruct (conf_state q1), (conf_state q2);
+             autorewrite with size' in H2, H3;
+             simpl in H2, H3;
+             Lia.lia.
+          -- unfold reads_left in H0; simpl in H0.
+             unfold configuration_room_left.
+             pose proof (conf_buf_sane q1).
+             rewrite Heqs in *.
+             autorewrite with size' in *;
+             simpl in H2; simpl;
+             destruct (conf_state q2);
+             try Lia.lia.
+        * destruct bs.
+          -- unfold reads_left in H0.
+             simpl in H0.
+             pose proof (conf_buf_sane q1).
+             pose proof (conf_buf_sane q2).
+             destruct (conf_state q1), (conf_state q2);
+             autorewrite with size' in *;
+             simpl in H2, H3;
+             Lia.lia.
+          -- autorewrite with follow.
+             eapply LeapsProofs.step_done in Heqs.
+             unfold conf_to_state_template.
+             rewrite follow_false.
+             erewrite buf_len_halted.
+             simpl.
+             left; reflexivity.
+             apply follow_false.
+             exact Heqs.
+             exact Heqs.
+      + rewrite <- H0.
+        simpl.
+        destruct (conf_state q2) eqn:?.
+        * rewrite <- Heqs.
+          apply foo.
+          split.
+          -- rewrite H0.
+             unfold reads_left; simpl.
+             pose proof (conf_buf_sane q1).
+             pose proof (conf_buf_sane q2).
+             destruct (conf_state q1), (conf_state q2);
+             autorewrite with size' in H2, H3;
+             simpl in H2, H3;
+             Lia.lia.
+          -- unfold reads_left in H0; simpl in H0.
+             unfold configuration_room_left.
+             pose proof (conf_buf_sane q2).
+             rewrite Heqs in *.
+             autorewrite with size' in *;
+             simpl in H2; simpl;
+             destruct (conf_state q1);
+             try Lia.lia.
+        * destruct bs.
+          -- unfold reads_left in H0.
+             simpl in H0.
+             pose proof (conf_buf_sane q1).
+             pose proof (conf_buf_sane q2).
+             destruct (conf_state q1), (conf_state q2);
+             autorewrite with size' in *;
+             simpl in H2, H3;
+             Lia.lia.
+          -- autorewrite with follow.
+             eapply LeapsProofs.step_done in Heqs.
+             unfold conf_to_state_template.
+             rewrite follow_false.
+             erewrite buf_len_halted.
+             simpl.
+             left; reflexivity.
+             apply follow_false.
+             exact Heqs.
+             exact Heqs.
+  Qed.
 
   Lemma wp_leaps_implies_bisim_leaps:
     forall q1 q2,
@@ -190,11 +562,16 @@ Section WPLeapsProofs.
         exact H2.
     - simpl interp_rels at 1.
       unfold follow_closed; intros.
-      clear H2; induction bs using rev_ind.
-      + autorewrite with follow; intuition.
-      + repeat rewrite follow_append.
-        apply top_closed.
-        apply IHbs.
+      apply top_closed.
+      rewrite H2.
+      unfold leap_size, reads_left.
+      simpl.
+      unfold configuration_room_left.
+      simpl.
+      unfold Reachability.S.
+      destruct (conf_state q0), (conf_state q3);
+      now autorewrite with size'.
+      intuition.
     - replace [] with (map (interp_conf_rel a) []) by reflexivity.
       now apply pre_bisimulation_embed.
   Qed.
